feat: fundamental app case

CollapsingTowers/TwoLevelBasic/SemEquiv.lean
@@ -9,6 +9,21 @@ def multi_subst : Subst → Expr → Expr
   | v :: γ, e => subst (γ.length) v (multi_subst γ e)
 
 @[simp]
+def multi_lc : Subst → Prop
+  | [] => true
+  | v :: γ => lc v ∧ multi_lc γ
+
+theorem multi_subst_lc : ∀ γ e, multi_lc γ → lc e → lc (multi_subst γ e) :=
+  by
+  intros γ e Hγ He
+  induction γ
+  case nil => apply He
+  case cons IH =>
+    rw [multi_subst]
+    apply subst_lc_at; apply Hγ.left
+    apply IH; apply Hγ.right
+
+@[simp]
 theorem multi_subst_app₁ : ∀ γ f arg, multi_subst γ (.app₁ f arg) = .app₁ (multi_subst γ f) (multi_subst γ arg) :=
   by
   intros γ f arg
@@ -16,7 +31,17 @@ theorem multi_subst_app₁ : ∀ γ f arg, multi_subst γ (.app₁ f arg) = .app
   case nil => rfl
   case cons IH => simp [IH]
 
+@[simp]
+theorem multi_subst_lit : ∀ γ n, multi_subst γ (.lit n) = .lit n :=
+  by
+  intros γ n
+  induction γ
+  case nil => rfl
+  case cons IH => simp [IH]
+
 mutual
+-- 𝓥⟦nat⟧ ≜ {(n, n) | n ∈ ℕ}
+-- 𝓥⟦τ𝕒 → τ𝕓⟧ ≜ {(λ.e₀, λ.e₁) | ∀ (v₀, v₁) ∈ 𝓥⟦τ𝕒⟧. lc (λ.e₀) ∧ lc (λ.e₁) ∧ (e₀⟦0/v₀⟧, e₁⟦0/v₁⟧) ∈ 𝓔⟦τ𝕓⟧}
 @[simp]
 def sem_equiv_value : Expr → Expr → Ty → Prop
   | .lit n₀, .lit n₁, .nat => n₀ = n₁
@@ -28,6 +53,7 @@ def sem_equiv_value : Expr → Expr → Ty → Prop
       sem_equiv_expr (open_subst v₀ e₀) (open_subst v₁ e₁) τ𝕓
   | _, _, _ => false
 
+-- 𝓔⟦τ⟧ ≜ {(e₀, e₁) | ∃v₀ v₁. e₀ ↦* v₀ ∧ e₁ ↦* v₁ ∧ (v₀, v₁) ∈ 𝓥⟦τ⟧}
 @[simp]
 def sem_equiv_expr (e₀ : Expr) (e₁ : Expr) (τ : Ty) : Prop :=
     ∃ v₀ v₁,
@@ -36,14 +62,15 @@ def sem_equiv_expr (e₀ : Expr) (e₁ : Expr) (τ : Ty) : Prop :=
       sem_equiv_value v₀ v₁ τ
 end
 
-@[simp]
-def sem_equiv_env : Subst → Subst → TEnv → Prop
-  | [], [], [] => true
-  | v₀ :: γ₀, v₁ :: γ₁, (τ, .stat) :: Γ =>
-    sem_equiv_value v₀ v₁ τ ∧
-    sem_equiv_env γ₀ γ₁ Γ
-  | _, _, _ => false
+inductive sem_equiv_env : Subst → Subst → TEnv → Prop where
+  | nil : sem_equiv_env [] [] []
+  | cons :
+    ∀ v₀ γ₀ v₁ γ₁ τ Γ,
+      sem_equiv_value v₀ v₁ τ →
+      sem_equiv_env γ₀ γ₁ Γ →
+      sem_equiv_env (v₀ :: γ₀) (v₁ :: γ₁) ((τ, .stat) :: Γ)
 
+-- Γ ⊧ e₀ ≈ e₁ : τ ≜ ∀ (γ₀, γ₁) ∈ 𝓖⟦Γ⟧. (γ₀(e₀), γ₁(e₁)) ∈ 𝓔⟦τ⟧
 @[simp]
 def sem_equiv_typing (Γ : TEnv) (e₀ : Expr) (e₁ : Expr) (τ : Ty) : Prop :=
   ∀ γ₀ γ₁,
@@ -71,6 +98,26 @@ theorem sem_equiv_value_impl_value :
     apply value.lam; apply Hlc₁
   all_goals simp at Hsem_value
 
+theorem sem_equiv_env_impl_multi_lc :
+  ∀ γ₀ γ₁ Γ,
+    sem_equiv_env γ₀ γ₁ Γ →
+    multi_lc γ₀ ∧
+    multi_lc γ₁ :=
+  by
+  intros γ₀ γ₁ Γ H
+  induction H
+  case nil => repeat constructor
+  case cons Hsem_value _ IH =>
+    constructor
+    . constructor
+      apply value_lc; apply And.left
+      apply sem_equiv_value_impl_value
+      apply Hsem_value; apply IH.left
+    . constructor
+      apply value_lc; apply And.right
+      apply sem_equiv_value_impl_value
+      apply Hsem_value; apply IH.right
+
 theorem sem_equiv_value_arrow_iff_lam :
   ∀ f₀ f₁ τ𝕒 τ𝕓,
     sem_equiv_value f₀ f₁ (.arrow τ𝕒 τ𝕓 .pure) →
@@ -95,6 +142,7 @@ theorem sem_equiv_expr_stepn :
   apply pure_stepn_trans; apply Hstepr₁ ; apply Hstepv₁
   apply Hsem_value
 
+-- Γ ⊢ e : τ → |Γ| ⊧ |e| ≈ |e| : |τ|
 theorem fundamental :
   ∀ Γ 𝕊 e τ φ,
     typing Γ 𝕊 e τ φ →
@@ -117,26 +165,95 @@ theorem fundamental :
     intros _ _ _ _ _ _ _ IH
     apply IH
   case app₁ =>
-    intros _ _ _ _ _ _ _ _ _ _ _ IHf IHarg
+    intros _ _ _ _ _ _ _ _ _ Hf Harg IHf IHarg
     intros γ₀ γ₁ semΓ
     simp only [sem_equiv_typing, sem_equiv_expr] at IHarg IHf
+    have ⟨Hmulti_lc₀, Hmulti_lc₁⟩ := sem_equiv_env_impl_multi_lc _ _ _ semΓ
     have ⟨v₀, v₁, Hstepv₀, Hstepv₁, Hsem_value⟩ := IHarg γ₀ γ₁ semΓ
+    have ⟨Hvalue₀, Hvalue₁⟩ := sem_equiv_value_impl_value _ _ _ Hsem_value
     have ⟨lam₀, lam₁, Hsteplam₀, Hsteplam₁, Hsem_value_lam⟩ := IHf γ₀ γ₁ semΓ
     have ⟨e₀, e₁, HEq₀, HEq₁⟩ := sem_equiv_value_arrow_iff_lam lam₀ lam₁ _ _ Hsem_value_lam
     rw [HEq₀, HEq₁, erase_ty, pure_empty, sem_equiv_value] at Hsem_value_lam
     have ⟨Hlc₀, Hlc₁, Hsem_value_lam⟩ := Hsem_value_lam
     apply sem_equiv_expr_stepn; apply Hsem_value_lam; apply Hsem_value
     . simp
+      -- left step
       apply pure_stepn_trans
       apply pure_stepn_at𝔹 _ _ _ (ctx𝔹.appl₁ _ _) Hsteplam₀
-      all_goals admit
-    . all_goals admit
+      apply multi_subst_lc; apply Hmulti_lc₀
+      apply erase_lc_at; apply typing_regular; apply Harg; rw [HEq₀]
+      -- right step
+      apply pure_stepn_trans
+      apply pure_stepn_at𝔹 _ _ _ (ctx𝔹.appr₁ _ _) Hstepv₀
+      apply value.lam; apply Hlc₀
+      -- head step
+      apply pure_stepn.multi; apply pure_stepn.refl
+      apply pure_step.pure_step𝕄 id; apply ctx𝕄.hole
+      constructor; apply Hlc₀; apply value_lc; apply Hvalue₀
+      apply head𝕄.app₁; apply Hvalue₀
+    . simp
+      -- left step
+      apply pure_stepn_trans
+      apply pure_stepn_at𝔹 _ _ _ (ctx𝔹.appl₁ _ _) Hsteplam₁
+      apply multi_subst_lc; apply Hmulti_lc₁
+      apply erase_lc_at; apply typing_regular; apply Harg; rw [HEq₁]
+      -- right step
+      apply pure_stepn_trans
+      apply pure_stepn_at𝔹 _ _ _ (ctx𝔹.appr₁ _ _) Hstepv₁
+      apply value.lam; apply Hlc₁
+      -- head step
+      apply pure_stepn.multi; apply pure_stepn.refl
+      apply pure_step.pure_step𝕄 id; apply ctx𝕄.hole
+      constructor; apply Hlc₁; apply value_lc; apply Hvalue₁
+      apply head𝕄.app₁; apply Hvalue₁
   case app₂ =>
-    intros _ _ _ _ _ _ _ _ _ IHf IHarg
-    admit
+    intros _ _ _ _ _ _ _ Hf Harg IHf IHarg
+    intros γ₀ γ₁ semΓ
+    simp only [sem_equiv_typing, sem_equiv_expr] at IHarg IHf
+    have ⟨Hmulti_lc₀, Hmulti_lc₁⟩ := sem_equiv_env_impl_multi_lc _ _ _ semΓ
+    have ⟨v₀, v₁, Hstepv₀, Hstepv₁, Hsem_value⟩ := IHarg γ₀ γ₁ semΓ
+    have ⟨Hvalue₀, Hvalue₁⟩ := sem_equiv_value_impl_value _ _ _ Hsem_value
+    have ⟨lam₀, lam₁, Hsteplam₀, Hsteplam₁, Hsem_value_lam⟩ := IHf γ₀ γ₁ semΓ
+    have ⟨e₀, e₁, HEq₀, HEq₁⟩ := sem_equiv_value_arrow_iff_lam lam₀ lam₁ _ _ Hsem_value_lam
+    rw [HEq₀, HEq₁, erase_ty, erase_ty, pure_empty, sem_equiv_value] at Hsem_value_lam
+    have ⟨Hlc₀, Hlc₁, Hsem_value_lam⟩ := Hsem_value_lam
+    apply sem_equiv_expr_stepn; apply Hsem_value_lam; apply Hsem_value
+    . simp
+      -- left step
+      apply pure_stepn_trans
+      apply pure_stepn_at𝔹 _ _ _ (ctx𝔹.appl₁ _ _) Hsteplam₀
+      apply multi_subst_lc; apply Hmulti_lc₀
+      apply erase_lc_at; apply typing_regular; apply Harg; rw [HEq₀]
+      -- right step
+      apply pure_stepn_trans
+      apply pure_stepn_at𝔹 _ _ _ (ctx𝔹.appr₁ _ _) Hstepv₀
+      apply value.lam; apply Hlc₀
+      -- head step
+      apply pure_stepn.multi; apply pure_stepn.refl
+      apply pure_step.pure_step𝕄 id; apply ctx𝕄.hole
+      constructor; apply Hlc₀; apply value_lc; apply Hvalue₀
+      apply head𝕄.app₁; apply Hvalue₀
+    . simp
+      -- left step
+      apply pure_stepn_trans
+      apply pure_stepn_at𝔹 _ _ _ (ctx𝔹.appl₁ _ _) Hsteplam₁
+      apply multi_subst_lc; apply Hmulti_lc₁
+      apply erase_lc_at; apply typing_regular; apply Harg; rw [HEq₁]
+      -- right step
+      apply pure_stepn_trans
+      apply pure_stepn_at𝔹 _ _ _ (ctx𝔹.appr₁ _ _) Hstepv₁
+      apply value.lam; apply Hlc₁
+      -- head step
+      apply pure_stepn.multi; apply pure_stepn.refl
+      apply pure_step.pure_step𝕄 id; apply ctx𝕄.hole
+      constructor; apply Hlc₁; apply value_lc; apply Hvalue₁
+      apply head𝕄.app₁; apply Hvalue₁
   case lit =>
-    intros _ _ _
-    admit
+    intros _ _ n
+    intros γ₀ γ₁ semΓ
+    simp only [sem_equiv_expr]
+    exists .lit n, .lit n
+    simp; apply pure_stepn.refl
   case lift_lit =>
     intros _ _ _ _ IH
     apply IH
